DY/Actions/ProtocolEvent.lean
@@ -1,0 +1,135 @@
+module
+
+public import DY.Trace
+public import DY.Bytes
+import DY.Step.Init
+import all DY.Trace
+public import DY.Step.Init
+import all DY.Step.Init
+
+namespace DY.ProtocolEvent
+
+public
+structure ExecEntryT (EventT: Type) where
+  ev: EventT
+
+public
+def baseAttackerKnowledge [BytesFunctor] [ExecTraceTypes] (EventT: Type): EntryBaseAttackerKnowledge (ExecEntryT EventT) where
+  attackerKnows _ _ _ := False
+
+public
+abbrev ProofEntryT (EventT: Type) := ExecEntryT EventT
+
+public
+def ProofEntryFunc (EventT: Type) := ProofEntryFun.default (ExecEntryT EventT)
+
+public
+class EventInv [TraceTypes] (EventT: Type) where
+  invariant: ProofTrace → EventT→ Prop
+
+public
+def Invariant [TraceTypes] (EventT: Type) [EventInv EventT]: TraceEntryInvariant (ProofEntryFunc EventT) where
+  invariant tr entry :=
+    EventInv.invariant tr entry.ev
+
+public
+theorem baseAttackerKnowledgeTheorem [TraceInvariant] [BytesFunctor] [BytesInvariants] (EventT: Type) [TraceTypes.Has (ProofEntryFunc EventT)] [EventInv EventT] [TraceInvariant.Has (Invariant EventT)]: EntryBaseAttackerKnowledgeTheorem (Invariant EventT) (baseAttackerKnowledge EventT) where
+  pf trBefore entry b := by
+    simp [baseAttackerKnowledge]
+
+public
+def _root_.DY.Trace.EventLoggedAt
+  {EventT: Type}
+  [ExecTraceTypes]
+  [ExecTraceTypes.Has (ExecEntryT EventT)]
+  (ev: EventT) (time: Nat)
+  (tr: ExecTrace)
+  : Prop
+:=
+  tr.at_is time (ExecEntryT.mk ev)
+
+public
+theorem _root_.DY.Trace.EventLoggedAt_le
+  {EventT: Type}
+  [ExecTraceTypes]
+  [ExecTraceTypes.Has (ExecEntryT EventT)]
+  (ev: EventT) (time: Nat)
+  (tr1 tr2: ExecTrace)
+  : tr1 ≤ tr2 →
+    tr1.EventLoggedAt ev time →
+    tr2.EventLoggedAt ev time
+:= by
+  grind [Trace.EventLoggedAt]
+
+grind_pattern Trace.EventLoggedAt_le => tr1 ≤ tr2, tr1.EventLoggedAt ev time
+
+public
+abbrev _root_.DY.Trace.EventLogged
+  {EventT: Type}
+  [ExecTraceTypes]
+  [ExecTraceTypes.Has (ExecEntryT EventT)]
+  (ev: EventT)
+  (tr: ExecTrace)
+  : Prop
+:=
+  ∃ i, tr.EventLoggedAt ev i
+
+public
+theorem _root_.DY.Trace.EventLoggedAt_imp_EventInv
+  {EventT: Type}
+  [TraceInvariant]
+  [EventInv EventT]
+  [TraceTypes.Has (ProofEntryFunc EventT)] [TraceInvariant.Has (Invariant EventT)]
+  (ev: EventT)
+  (i: Nat)
+  (tr: ProofTrace)
+  : tr.Invariant →
+    tr.erase.EventLoggedAt ev i →
+    EventInv.invariant (tr.prefix i) ev
+:= by
+  intro h_inv h_ev
+  have := Trace.invariant_at tr i (by grind [Trace.EventLoggedAt, Trace.at_is]) h_inv
+  suffices (Invariant EventT).invariant (tr.prefix i) (ExecEntryT.mk ev) by
+    simp_all [Invariant]
+  rewrite [← TraceInvariant.Has.inv_commutes]
+  simp [Trace.EventLoggedAt, Trace.at_is, IntoTraceEntry.make, Trace.erase_at] at h_ev
+  grind
+
+public
+def logEvent
+  {EventT: Type}
+  [ExecTraceTypes]
+  [ExecTraceTypes.Has (ExecEntryT EventT)]
+  (ev: EventT): Traceful Unit
+:= do
+  let entry: ExecEntryT EventT := { ev }
+  let _i ← appendEntry entry
+  return ()
+
+@[instance]
+public
+theorem logEvent.spec
+  {EventT: Type}
+  [TraceInvariant]
+  [EventInv EventT]
+  [TraceTypes.Has (ProofEntryFunc EventT)] [TraceInvariant.Has (Invariant EventT)]
+  (ev: EventT)
+  : HoareTriple
+    (logEvent ev)
+    (fun tr => EventInv.invariant tr ev)
+    (fun _ tr => tr.erase.EventLogged ev)
+:= by
+  apply HoareTriple.mk
+  unfold logEvent
+  dsimp only
+  unfold hoareTriple
+  intro tr h_pre h_inv
+  mark_non_monotone h_pre
+  step with ⟨ ExecEntryT.mk ev ⟩ by simp_all [ProofEntryFunc, Invariant]
+  step
+  simp only [Trace.EventLogged, Trace.EventLoggedAt]
+  exists _i
+  have := Trace.at_is_erase tr _i (ExecEntryT.mk ev)
+  grind [ProofEntryFunc]
+
+end DY.ProtocolEvent
